code/ecdsap256sha2/Hacl.Impl.P256.Compression.fst
@@ -1,0 +1,16 @@
+module Hacl.Impl.P256.Compression
+
+open FStar.HyperStack.All
+open FStar.HyperStack
+module ST = FStar.HyperStack.ST
+
+open Lib.IntTypes
+open Lib.Buffer
+
+open Spec.P256.Definitions
+
+let decompressionNotCompressed b result = 
+  (u64 0)
+
+let decompressionCompressed b result = 
+  (u64 0)
