code/ecdsap256sha2/Hacl.Impl.P256.Compression.fsti
@@ -1,0 +1,23 @@
+module Hacl.Impl.P256.Compression
+
+open FStar.HyperStack.All
+open FStar.HyperStack
+module ST = FStar.HyperStack.ST
+
+open Lib.IntTypes
+open Lib.Buffer
+
+open Spec.P256.Definitions
+
+
+let notCompressedForm = lbuffer uint8 (size 64)
+let compressedForm = lbuffer uint8 (size 64)
+
+(* the name makes a lot of sense, doesnot it? *)
+val decompressionNotCompressed: notCompressedForm -> result: point -> Stack bool 
+  (requires fun h -> True)
+  (ensures fun h0 _ h1 -> True)
+
+val decompressionCompressed: compressedForm -> result: point -> Stack bool 
+  (requires fun h -> True)
+  (ensures fun h0 _ h1 -> True)
